---
layout: post
title: "高概HW2"
date: 2024-10-16
categories: [数学好难]
tags: []  
---

## Question 1

(i) Denote $r = \sqrt{X^2+Y^2}$ and $\theta = \arcsin \frac{Y}{X}$.

　Then we have $U = r^2$ and $V = \cos \theta $.

　$f_{XY}(x, y)=\frac{1}{2\pi} \exp (-\frac{x^2+y^2}{2})=\frac{1}{2\pi} \exp (-\frac{r^2}{2})$

　$\frac{1}{J} = \begin{vmatrix} \frac{\partial x}{\partial r}&\frac{\partial x}{\partial \theta}\\
　\frac{\partial y}{\partial r}&\frac{\partial y}{\partial \theta}  \end{vmatrix} = r$

　$f_{R\theta}(r, \theta) = f_{XY}(x, y)\cdot \frac{1}{\mid J\mid } = \frac{r}{2\pi} \exp (-\frac{r^2}{2})$

　since $R = \sqrt{U}$ and $\theta = \arccos V$,

　The Jacobian for the transformation from $(R, \theta)$ to $(U, V)$ should be

　$J' = \begin{vmatrix} \frac{\partial u}{\partial r}&\frac{\partial u}{\partial \theta}\\
　\frac{\partial v}{\partial r}&\frac{\partial v}{\partial \theta}  \end{vmatrix} = -2r\cdot \frac{1}{\sqrt{1-v^2}}$

　$f_{UV}(u, v)=\frac{u}{\pi \sqrt{1-v^2}} e^{-\frac{u}{2}}, u\geq 0, -1\leq v \leq 1$.

(ii) $f_U(u) = \int _{-1}^1 \frac{u}{\pi \sqrt{1-v^2}} e^{-\frac{u}{2}} \mathrm dv = ue^{-\frac{u}{2}}, u\geq 0$

　$f_V(v) = \int _0^{+\infty} \frac{u}{\pi \sqrt{1-v^2}} e^{-\frac{u}{2}} \mathrm du =\frac{2}{\pi \sqrt{1-v^2}}, -1\leq v \leq 1$

　since $f_{UV}(u, v) = f_U(u)\cdot f_V(v)$, U and V are independent.

## Question 2

　(i) since X and Y are independent, we have

　$f_{XY}(x, y) = f_X(x)\cdot f_Y(y)=\frac{e^{-\lambda_1}\lambda_1^x}{x!}\cdot \frac{e^{-\lambda_2}\lambda_2^y}{y!}$.

　$P(X=x \mid X+Y=n) = \frac{P(X=x, Y=n-x)}{P(X+Y=n)}$

　$P(X = x \mid X + Y = n) = \frac{\frac{e^{-\lambda_1} \lambda_1^x}{x!} \cdot \frac{e^{-\lambda_2} \lambda_2^{n-x}}{(n-x)!}}{\frac{e^{-(\lambda_1 + \lambda_2)} (\lambda_1 + \lambda_2)^n}{n!}}$

　Simplify the expression:

　$P(X = x \mid X + Y = n) = \frac{e^{-\lambda_1} \lambda_1^x e^{-\lambda_2} \lambda_2^{n-x} n!}{x! (n-x)! e^{-(\lambda_1 + \lambda_2)} (\lambda_1 + \lambda_2)^n}$

　$P(X = x \mid X + Y = n) = \frac{n!}{x! (n-x)!} \cdot \frac{\lambda_1^x \lambda_2^{n-x}}{(\lambda_1 + \lambda_2)^n}$
　
　Therefore, $P(X = x \mid X + Y = n) \sim B(n, \frac{\lambda_1}{\lambda_1 + \lambda_2})$.



## Question 3

(i) $Y \mid  X=x \sim U(-\sqrt{1-x^2}, \sqrt{1-x^2})$

　Therefore, $f_{y\mid x}(Y\mid X=x)=\frac{1}{2\sqrt{1-x^2}}, y\in (-\sqrt{1-x^2}, \sqrt{1-x^2})$.

(ii) $f_{y\mid x}(Y\mid X=0)=1/2$

　Therefore, $P(Y>0\mid X=0)=\int_{-1}^0 1/2\  \mathrm dy=1/2$.

## Question 4

　since we have $h_1(g_1(x, y), g_2(x, y)) = x$,

　Then $\frac{\partial {h_1}}{\partial {g_1}} \frac{\partial g_1}{\partial x} + \frac{\partial {h_1}}{\partial {g_2}} \frac{\partial g_2}{\partial x} = 1$

　Which is $\frac{\partial {h_1}}{\partial {u}} \frac{\partial  g_1}{\partial  x} + \frac{\partial {h_1}}{\partial {v}} \frac{\partial  g_2}{\partial x} = 1$

　Similarly we have

　$\frac{\partial {h_1}}{\partial {u}} \frac{\partial  g_1}{\partial  y} + \frac{\partial {h_1}}{\partial { v}} \frac{\partial  g_2}{\partial y} = 0$

　$\frac{\partial {h_2}}{\partial {u}} \frac{\partial  g_1}{\partial  x} + \frac{\partial {h_2}}{\partial {v}} \frac{\partial  g_2}{\partial x} = 0$

　$\frac{\partial {h_2}}{\partial {u}} \frac{\partial  g_1}{\partial  y} + \frac{\partial {h_2}}{\partial {v}} \frac{\partial   g_2}{\partial y} = 1$

　It can be observed that these four equations can be derived from a linear equation system, which is

　$\begin{pmatrix}
\frac{\partial h_1}{\partial u} & \frac{\partial h_1}{\partial v} \\
\frac{\partial h_2}{\partial u} & \frac{\partial h_2}{\partial v}
　\end{pmatrix} \cdot 
　\begin{pmatrix}
\frac{\partial g_1}{\partial x} & \frac{\partial g_1}{\partial y} \\
\frac{\partial g_2}{\partial x} & \frac{\partial g_2}{\partial y}
　\end{pmatrix}
　=
　\begin{pmatrix}
　1 \ 0 \\
　0 \ 1
　\end{pmatrix}$

　Since $J_{UV}(x, y)$ is invertible, multiple the two sides by $J_{UV}^{-1}(x, y)$ and we have

　$J_{XY}(u, v)=J_{UV}^{-1}(x, y)$.
　
　
　
## Question 5
　
(i) $F_U(u) = P(U\leq u) = \int_0^u{f_X(x)}\int_0^{+\infty}{f_Y(y)}\mathrm dx\mathrm dy + \int_u^{+\infty}{f_X(x)}\int_0^u{f_Y(y)}\mathrm dx\mathrm dy$

　$= (1-e^{-\lambda u})+e^{-\lambda u}(1-e^{-\lambda u})$

　$=1-e^{-2\lambda u}$. Therefore $U \sim \mathrm{exp}(2)$.

(ii) $F_V(v) = P(V\leq v) = \int_0^v{f_X(x)}\int_0^v{f_Y(y)}\mathrm dx\mathrm dy$

　$=1-2e^{-\lambda v}+e^{-2\lambda v}, v\geq 0$.

　Denote $W = X + \frac{1}{2}Y \in (0, \infty)$.

　$F_W(w)=\int_{x=0}^w\int_{y=0}^{2(w-x)}f_Y(y)\mathrm dyf_X(x)\mathrm dx$

　$=\int_{x=0}^w\lambda e^{-\lambda x}(1-e^{-2\lambda (w-x)}) \mathrm dx$

　$=\int_{x=0}^w\lambda e^{-\lambda x}\mathrm dx - \int_{x=0}^w\lambda e^{-\lambda x}e^{-2\lambda (w-x)} \mathrm dx$

　$=1-e^{-\lambda w} -e^{-\lambda w} +e^{-2\lambda w}$

　$=1-2e^{-\lambda w} +e^{-2\lambda w} = F_V(v)$.

　Therefore, $V$ has the same distribution as $X+\frac{1}{2}Y$.

　(iii) Since $V$ has the same distribution with $X+\frac{1}{2} Y$,

　We have $E(V)=E(X)+0.5E(Y)=3\lambda /2$ 

　and $Var(V) = Var(X)+(1/2)^2Var(Y)=4\lambda/5$.
　
　
